WiP: proving main lemma, about to include init_tls in tc_enum

src/travorder/TravOrderConfig.v
@@ -1244,4 +1244,127 @@ Proof using.
   clear. unfolder; ins; do 2 desf.
 Admitted.
   
+(* Require Import Set2TravConfig. *)
+Section Traversal.
+  Variable (steps: nat -> trav_label).
+  Hypothesis (ENUM: enumerates steps (exec_tls G)).
+  Hypothesis (RESP: respects_rel steps (iord G sc)⁺ (exec_tls G)).
+  
+  Definition tc_enum (i: nat): trav_label -> Prop  :=
+    sim_clos (trav_prefix steps i).
+  
+  Lemma trav_prefix_init:
+    trav_prefix steps 0 ≡₁ ∅. 
+  Proof.
+    unfold trav_prefix. apply set_subset_empty_r, set_subset_bunion_l.
+    ins. lia. 
+  Qed.
+  
+  Ltac liaW no := destruct no; [done| ins; lia]. 
+  
+  Lemma trav_prefix_iord_coherent 
+        (i : nat) (DOMi: NOmega.le (NOnum i) (set_size (exec_tls G))):
+    iord_coherent G sc (trav_prefix steps i).
+  Proof using RESP ENUM.
+    induction i.
+    { rewrite trav_prefix_init. red. basic_solver. }
+    rewrite trav_prefix_ext; eauto. red.
+    rewrite id_union, seq_union_r, dom_union.
+    apply set_subset_union_l. split. 
+    { unfold iord_coherent in IHi. rewrite IHi; [basic_solver| ].
+      liaW (set_size (exec_tls G)). }
+    red. intros tlj. intros [tli IORD%seq_eqv_r]. desc.
+    apply iord_exec_tls in IORD. red in IORD. desc.
+    apply enumeratesE' in ENUM. cdes ENUM.
+    apply IND in IORD1, IORD2. desc. rename i1 into j.
+    assert (i0 = i) as -> by (apply INJ; auto; congruence).
+    subst. 
+    pose proof (Nat.lt_trichotomy i j) as LT. des; revgoals. 
+    { left. red. vauto. }
+    { subst. basic_solver. }
+    enough (j < i); [lia| ]. eapply RESP; eauto. 
+  Qed.
+  
+  Lemma trav_prefix_step
+        i (DOMsi: NOmega.lt_nat_l i (set_size (exec_tls G))):
+    iord_step (trav_prefix steps i) (trav_prefix steps (S i)).
+  Proof using RESP ENUM.
+    red. exists (steps i). do 2 red.
+    splits; try by (apply trav_prefix_iord_coherent; liaW (set_size (exec_tls G))).
+    apply seq_eqv_l. split.
+    { eapply prefix_border; eauto. }
+    eapply trav_prefix_ext; eauto. 
+  Qed.
+  
+  Lemma sim_traversal_next WF CONS:
+    forall i (DOMi: NOmega.lt_nat_l i (set_size (exec_tls G))),
+      (* (sim_trav_step G sc)^* (tc_enum i) (tc_enum (1 + i)). *)
+      (sim_clos_step^*) (tc_enum i) (tc_enum (1 + i)). 
+  Proof using RESP ENUM.
+    ins. unfold tc_enum. 
+    apply iord_step_implies_sim_clos_step; auto.
+    apply trav_prefix_step; auto. 
+  Qed.
+
+  (* Lemma init_tc_enum: *)
+  (*   tc_enum 0 = init_tls G.  *)
+  (* Proof.  *)
+  (*   unfold tc_enum, init_tls, sim_clos.  *)
+
+
+End Traversal.
+
+
+(* TODO: rename *)
+Lemma sim_traversal_inf WF CONS
+      (FAIR: mem_fair G)
+      (IMM_FAIR: imm_s_fair G sc)
+  :
+  exists (sim_enum: nat -> (trav_label -> Prop)),
+    ⟪INIT: sim_enum 0 = init_tls G ⟫ /\
+      (* ⟪DOM_TC: forall i (DOMi: NOmega.le (NOnum i) (set_size (exec_tls G))), *)
+      (*     covered (sim_enum i) ⊆₁ E /\ issued (sim_enum i) ⊆₁ E ⟫ /\ *)
+      (* ⟪COH: forall i (DOMi: NOmega.le (NOnum i) (set_size (graph_steps G))), *)
+      (*     tc_coherent G sc (sim_enum i) ⟫ /\ *)
+      ⟪COH: forall i (DOMi: NOmega.le (NOnum i) (set_size (exec_tls G))),
+          tls_coherent G (sim_enum i)⟫ /\
+      ⟪STEPS: forall i (DOMi: NOmega.lt_nat_l i (set_size (exec_tls G))),
+          (sim_clos_step^*) (sim_enum i) (sim_enum (1 + i)) ⟫ /\
+      ⟪ENUM: forall e (Ee: (E \₁ is_init) e), exists i,
+          NOmega.le (NOnum i) (set_size (exec_tls G)) /\
+            (sim_enum i) (mkTL ta_cover e)⟫.
+Proof using.
+  edestruct iord_enum_exists as [steps_enum [ENUM RESP]]; eauto.
+  1, 2: by apply CONS.
+  exists (tc_enum steps_enum). splits.
+  {p unfold tc_enum, init_tls. 
+
+
+
+
+  
+  { unfold tc_enum, trav_prefix. rewrite <- sim_trav_closure_init; auto. f_equal.
+    apply same_tc_extensionality.
+    arewrite ((fun i => i < 0) ≡₁ (@set_empty nat)).
+    { split; [red; ins; lia| basic_solver]. }
+    rewrite set_bunion_empty. by rewrite set2trav_config_empty. }
+  3: { apply sim_traversal_next; auto. }
+  2: { ins. unfold tc_enum. apply stc_coherent; auto.
+       apply tc_coherent_alt_implies_tc_coherent, trav_prefix_coherent_alt; auto. }
+  { intros i DOM. unfold tc_enum. eapply stc_domE; eauto.
+    1, 2: unfold set2trav_config; simpl; basic_solver.
+    apply tc_coherent_alt_implies_tc_coherent, trav_prefix_coherent_alt; auto. }
+  intros e Ee.
+  pose proof ENUM as ENUM'. apply enumeratesE' in ENUM. desc.
+  specialize (IND (mkTL ta_cover e)). specialize_full IND; [by vauto| ].
+  desc. exists (S i). split; [by vauto| ].
+  unfold tc_enum, sim_trav_closure.
+  unfold trav_config_union. simpl. left. split; [| by apply Ee].
+  left. split; [| by apply Ee].
+  exists (mkTL ta_cover e). split; auto. split; [by vauto| ].
+  rewrite <- IND0. eapply trav_prefix_ext; eauto. basic_solver.
+Qed.
+
+
 End TravOrderConfig.
+  
